Add regions

CC/Context.lean
@@ -4,43 +4,62 @@ import CC.Type
 
 namespace CC
 
+inductive Region : Nat -> Type where
+| var : Fin n -> Region n
+| glob : Region n
+
+def Region.rename (r : Region n1) (f : VarMap n1 n2) : Region n2 :=
+  match r with
+  | Region.var x => Region.var (f x)
+  | Region.glob => Region.glob
+
+def Region.weaken_var (r : Region n) : Region n.succ :=
+  r.rename weaken_map
+
+def Region.weaken_var1 (r : Region (Nat.succ n)) : Region (Nat.succ n).succ :=
+  r.rename weaken_map.ext
+
+def Region.weaken_var_glob_def :
+  (Region.glob : Region n).weaken_var = Region.glob := by rfl
+
 inductive Ctx : Nat -> Nat -> Type where
 | empty : Ctx 0 0
 | extend_var :
   Ctx n m ->
   CType n m ->
+  Region n ->
   Ctx n.succ m
 | extend_tvar :
   Ctx n m ->
   PType n m ->
   Ctx n m.succ
 
-inductive BoundVar : Ctx n m -> Fin n -> CType n m -> Prop where
+inductive BoundVar : Ctx n m -> Fin n -> CType n m -> Region n -> Prop where
 | here :
-  BoundVar (Ctx.extend_var Γ T) 0 T.weaken_var
+  BoundVar (Ctx.extend_var Γ T r) 0 T.weaken_var r.weaken_var
 | there_var :
-  BoundVar Γ x T ->
-  BoundVar (Ctx.extend_var Γ T') x.succ T.weaken_var
+  BoundVar Γ x T r ->
+  BoundVar (Ctx.extend_var Γ T' r') x.succ T.weaken_var r.weaken_var
 | there_tvar :
-  BoundVar Γ x T ->
-  BoundVar (Ctx.extend_tvar Γ S) x T.weaken_tvar
+  BoundVar Γ x T r ->
+  BoundVar (Ctx.extend_tvar Γ S) x T.weaken_tvar r
 
 inductive BoundTVar : Ctx n m -> Fin m -> PType n m -> Prop where
 | here :
   BoundTVar (Ctx.extend_tvar Γ S) 0 S.weaken_tvar
 | there_var :
   BoundTVar Γ x S ->
-  BoundTVar (Ctx.extend_var Γ T) x S.weaken_var
+  BoundTVar (Ctx.extend_var Γ T r) x S.weaken_var
 | there_tvar :
   BoundTVar Γ x S ->
   BoundTVar (Ctx.extend_tvar Γ S') x.succ S.weaken_tvar
 
 def BoundVar.pred'
   {Γ : Ctx n m} {P : CType n m} {T : CType n.succ m} :
-  Γ0 = Ctx.extend_var Γ P ->
+  Γ0 = Ctx.extend_var Γ P p ->
   x0 = x.succ ->
-  BoundVar Γ0 x0 T ->
-  ∃ T0, T = T0.weaken_var ∧ BoundVar Γ x T0 := by
+  BoundVar Γ0 x0 T r ->
+  ∃ T0 r0, T = T0.weaken_var ∧ r = r0.weaken_var ∧ BoundVar Γ x T0 r0 := by
   intro he1 he2 h
   cases h <;> try (solve | cases he1 | cases he2)
   cases he1
@@ -50,7 +69,19 @@ def BoundVar.pred'
 
 def BoundVar.pred
   {Γ : Ctx n m} {P : CType n m} {T : CType n.succ m} :
-  BoundVar (Ctx.extend_var Γ P) x.succ T ->
-  ∃ T0, T = T0.weaken_var ∧ BoundVar Γ x T0 := by
+  BoundVar (Ctx.extend_var Γ P p) x.succ T r ->
+  ∃ T0 r0, T = T0.weaken_var ∧ r = r0.weaken_var ∧ BoundVar Γ x T0 r0 := by
   intro h
   apply BoundVar.pred' <;> aesop
+
+@[simp]
+def Region.rename_id {r : Region n} :
+  r.rename id = r := by
+  cases r <;> rfl
+
+theorem Region.rename_comp {r : Region n} :
+  (r.rename f1).rename f2 = r.rename (f2.comp f1) := by
+  cases r <;> unfold VarMap.comp <;> simp [rename]
+
+lemma Region.weaken_var1_def {r : Region (Nat.succ n)} :
+  r.weaken_var1 = r.rename weaken_map.ext := by simp [weaken_var1]
