CC/Typed.lean
@@ -23,7 +23,7 @@ def Variance.neg : Variance -> Variance
 
 inductive RefineCaptureSet : CaptureSet n -> Fin n -> Variance -> CaptureSet n -> Prop where
 | pos :
-  RefineCaptureSet ⟨cs, rs, u⟩ x Variance.cov ⟨∅, rs ∪ {x}, false⟩
+  RefineCaptureSet ⟨cs, rs, u⟩ x Variance.cov ⟨∅, {x}, false⟩
 | neg :
   RefineCaptureSet ⟨cs, rs, u⟩ x Variance.cot ⟨cs, rs, u⟩
 
@@ -53,7 +53,7 @@ inductive DropBinder : CaptureSet n.succ -> CaptureSet n -> Prop where
 
 inductive Typed : Ctx n m -> Term n m -> CaptureSet n -> CType n m -> Prop where
 | var :
-  BoundVar Γ x (CType.capt C S) ->
+  BoundVar Γ x (CType.capt C S) r ->
   Typed Γ (Term.var x) {x} (CType.capt {x} S)
 | var_refine :
   Typed Γ (Term.var x) {x} (CType.capt C S) ->
@@ -64,7 +64,7 @@ inductive Typed : Ctx n m -> Term n m -> CaptureSet n -> CType n m -> Prop where
   Subtype Γ T T' ->
   Typed Γ t C T'
 | abs :
-  Typed (Ctx.extend_var Γ T) t C U ->
+  Typed (Ctx.extend_var Γ T Region.glob) t C U ->
   DropBinder C C' ->
   Typed Γ (Term.abs T t) C' (CType.capt C' (PType.arr T U))
 | tabs :
@@ -85,14 +85,14 @@ inductive Typed : Ctx n m -> Term n m -> CaptureSet n -> CType n m -> Prop where
   Typed Γ (Term.unbox C x) (C ∪ {x}) (CType.capt C S)
 | letval1 : ∀ {Γ : Ctx n m} {U' : CType n m} {Cu' : CaptureSet n},
   Typed Γ t Ct T ->
-  Typed (Ctx.extend_var Γ T) u Cu U ->
+  Typed (Ctx.extend_var Γ T Region.glob) u Cu U ->
   U = U'.weaken_var ->
   DropBinder Cu Cu' ->
   Typed Γ (Term.letval t u) (Ct ∪ Cu') U'
 | letval2 : ∀ {Γ : Ctx n m} {U' : CType n m} {Cu' : CaptureSet n},
   Typed Γ v Ct T ->
   Value v ->
-  Typed (Ctx.extend_var Γ T) u Cu U ->
+  Typed (Ctx.extend_var Γ T Region.glob) u Cu U ->
   U = U'.weaken_var ->
   DropBinderFree Cu Cu' ->
   Typed Γ (Term.letval v u) Cu' U'
